---
id: Q1_extra
title: Q1 Extra
sidebar_position: 2
---

# 

### Response Calculation when $$D(z) = 2 - z^{-1}$$:

$$
Y(z) = R(z) \cdot D(z) \cdot G(z)
$$

Therefore, $$Y(z)$$ is:

$$
Y(z) = \frac{z}{z - 1} \cdot (2 - z^{-1}) \cdot \frac{0.1(z + 1)}{(z-1)(z-0.6)}
$$

$$
Y(z) = \frac{z}{z - 1} \cdot \frac{2z - 1}{z} \cdot \frac{0.1(z + 1)}{(z-1)(z-0.6)}
$$

$$
Y(z) = \frac{0.1(2z - 1)(z + 1)}{(z - 1)^2(z-0.6)}
$$

**Partial Fraction Decomposition of $$Y(z)$$:**

To simplify the process, we'll first find the partial fraction decomposition of $$Y(z)/z$$:

$$
\frac{Y(z)}{z} = \frac{0.1 \cdot (2z - 1) \cdot (z + 1)}{z \cdot (z - 1)^2 \cdot (z - 0.6)}
$$


$$
\frac{Y(z)}{z} = \frac{A}{z} + \frac{B}{z - 1} + \frac{C}{(z - 1)^2} + \frac{D}{z - 0.6}
$$


Multiplying both sides by $$z(z - 1)^2(z - 0.6)$$:

$$
0.1 \cdot (2z - 1) \cdot (z + 1) = A(z - 1)^2(z - 0.6) + Bz(z - 1)(z - 0.6) + Cz(z - 0.6) + Dz(z - 1)^2
$$


*   **Let $$z = 0$$:**
    <div style={{display:"block", paddingLeft: "2rem"}}>
    $$0.1 \cdot (-1) \cdot (1) = A(-1)^2(-0.6)$$
    </div>
    <div style={{display:"block", paddingLeft: "2rem"}}>
    $$-0.1 = -0.6A$$
    </div>
    <div style={{display:"block", paddingLeft: "2rem"}}>
    $$A = \frac{1}{6}$$
    </div>

*   **Let $$z = 1$$:**
    <div style={{display:"block", paddingLeft: "2rem"}}>
    $$0.1 \cdot (1) \cdot (2) = C(1)(0.4)$$
    </div>
    <div style={{display:"block", paddingLeft: "2rem"}}>
    $$0.2 = 0.4C$$
    </div>
    <div style={{display:"block", paddingLeft: "2rem"}}>
    $$C = 0.5$$
    </div>

*   **Let $$z = 0.6$$:**
    <div style={{display:"block", paddingLeft: "2rem"}}>
    $$0.1 \cdot (0.2) \cdot (1.6) = D(0.6)(-0.4)^2$$
    </div>
    <div style={{display:"block", paddingLeft: "2rem"}}>
    $$0.032 = 0.096D$$
    </div>
    <div style={{display:"block", paddingLeft: "2rem"}}>
    $$D = \frac{1}{3}$$
    </div>

*   **To find $$B$$, we can equate coefficients of $$z^3$$ on both sides or substitute another value of $$z$$. Let's equate coefficients of $$z^3$$**
    <div style={{display:"block", paddingLeft: "2rem"}}>
    $$0.1 \cdot 2 = A + B + D$$
    </div>
    <div style={{display:"block", paddingLeft: "2rem"}}>
    $$0.2 = \frac{1}{6} + B + \frac{1}{3}$$
    </div>
    <div style={{display:"block", paddingLeft: "2rem"}}>
    $$B = -0.3$$
    </div>

**Substitute the Constants Back into $$Y(z)/z$$**


$$
\frac{Y(z)}{z} = \frac{(1/6)}{z} - \frac{0.3}{z - 1} + \frac{0.5}{(z - 1)^2} + \frac{(1/3)}{z - 0.6}
$$

Multiply both sides by $$z$$ to get $$Y(z)$$:

$$
Y(z) = \frac{1}{6} - \frac{0.3z}{z - 1} + \frac{0.5z}{(z - 1)^2} + \frac{(1/3)z}{z - 0.6}
$$

**Take the Inverse Z-Transform**

$$
y[n] = \frac{1}{6}\delta[n] - 0.3u[n] + 0.5nu[n] + \frac{1}{3}(0.6)^n u[n]
$$

:::tip
*   $$\mathcal{Z}^{-1}\left\{\frac{1}{6}\right\} = \frac{1}{6}\delta[n]$$
*   $$\mathcal{Z}^{-1}\left\{\frac{z}{z - 1}\right\} = u[n]$$
*   $$\mathcal{Z}^{-1}\left\{\frac{z}{(z - 1)^2}\right\} = n \cdot u[n]$$
*   $$\mathcal{Z}^{-1}\left\{\frac{z}{z - a}\right\} = a^n \cdot u[n]$$
:::