---
id: Q5
title: Q5
---

#


Find the z-transform of 
$$
\frac{1}{s^2(s+1)}
$$

We decompose $$\frac{1}{s^{2}(s + 1)}$$ using partial fractions:

$$
\frac{1}{s^{2}(s + 1)} = \frac{A}{s} + \frac{B}{s^{2}} + \frac{C}{s + 1}
$$

To find A, B, and C:

*   **Set s = 0:**
    <div style={{display:"block", paddingLeft: "2rem"}}>
    $$1 = A(0)(0 + 1) + B(0 + 1) + C(0)^{2}$$
    </div>
    <div style={{display:"block", paddingLeft: "2rem"}}>
    $$B = 1$$
    </div>

*   **Set s = -1:**
    <div style={{display:"block", paddingLeft: "2rem"}}>
    $$1 = A(-1)(-1 + 1) + B(-1 + 1) + C(-1)^{2}$$
    </div>
    <div style={{display:"block", paddingLeft: "2rem"}}>
    $$C = 1$$
    </div>

*   **Set s = 1:**
    <div style={{display:"block", paddingLeft: "2rem"}}>
    $$1 = A(1)(1 + 1) + B(1 + 1) + C(1)^{2}$$
    </div>
    <div style={{display:"block", paddingLeft: "2rem"}}>
    $$1 = 2A + 2 + 1$$
    </div>
    <div style={{display:"block", paddingLeft: "2rem"}}>
    $$A = -1$$
    </div>

Therefore:

$$
\frac{1}{s^{2}(s + 1)} = -\frac{1}{s} + \frac{1}{s^{2}} + \frac{1}{s + 1}
$$

$$
\mathcal{L}^{-1}\Bigl\{\frac{1}{s^{2}(s + 1)}\Bigr\} = -1 + t + e^{-t}
$$

$$
Z\{-1 + t + e^{-t}\} = -\frac{z}{z - 1} + \frac{Tz}{(z - 1)^{2}} + \frac{z}{z - e^{-T}}
$$
